ulib/FStar.Tactics.fst
@@ -58,33 +58,29 @@ type term_view =
   (* TODO: complete *)
 
 
-noeq type _result (a:Type) =
-  | Success: a -> state -> _result a
-  | Failed: string -> state -> _result a
+noeq type __result (a:Type) =
+  | Success: a -> state -> __result a
+  | Failed: string -> state -> __result a
 
 (* If it starts with an underline don't use it from the outside! *)
 
-let _tac (a:Type) = state -> M (_result a)
+let __tac (a:Type) = state -> M (__result a)
 
 (* monadic return *)
-val _ret : a:Type -> x:a -> _tac a
-let _ret a x = fun (s:state) -> Success x s
+val __ret : a:Type -> x:a -> __tac a
+let __ret a x = fun (s:state) -> Success x s
 
 (* monadic bind *)
-let _bind (a:Type) (b:Type) 
-         (t1:_tac a)
-         (t2:a -> _tac b)
-    : _tac b
-    = fun p ->
-        let r = t1 p in
-        match r with
-        | Success a q  -> t2 a q
-        | Failed msg q -> Failed msg q
+let __bind (a:Type) (b:Type) (t1:__tac a) (t2:a -> __tac b) : __tac b =
+    fun p -> let r = t1 p in
+             match r with
+             | Success a q  -> t2 a q
+             | Failed msg q -> Failed msg q
 
 (* Actions *)
-let _get () : _tac state = fun s0 -> Success s0 s0 
+let __get () : __tac state = fun s0 -> Success s0 s0 
 
-let tac_wp a = state -> (_result a -> Tot Type0) -> Tot Type0
+let tac_wp a = state -> (__result a -> Tot Type0) -> Tot Type0
 
 (*
  * The DMFF-generated `bind_wp` doesn't the contain the "don't duplicate the post-condition"
@@ -98,7 +94,7 @@ unfold let g_bind (a:Type) (b:Type) (wp:tac_wp a) (f:a -> tac_wp b) = fun ps pos
                      | Failed msg q -> post (Failed msg q))
 
 unfold let g_compact (a:Type) (wp:tac_wp a) : tac_wp a =
-    fun ps post -> wp ps (fun _ -> True) /\ (forall (r:_result a). post r \/ wp ps (fun r' -> ~(r == r')))
+    fun ps post -> wp ps (fun _ -> True) /\ (forall (r:__result a). post r \/ wp ps (fun r' -> ~(r == r')))
 
 unfold let __TAC_eff_override_bind_wp (r:range) (a:Type) (b:Type) (wp:tac_wp a) (f:a -> tac_wp b) =
     g_compact b (g_bind a b wp f)
@@ -106,17 +102,17 @@ unfold let __TAC_eff_override_bind_wp (r:range) (a:Type) (b:Type) (wp:tac_wp a) 
 (* total  *) //disable the termination check, although it remains reifiable
 reifiable reflectable new_effect {
   TAC : a:Type -> Effect
-  with repr     = _tac
-     ; bind     = _bind
-     ; return   = _ret
-     ; _get     = _get
+  with repr     = __tac
+     ; bind     = __bind
+     ; return   = __ret
+     ; __get    = __get
 }
 effect Tac (a:Type) = TAC a (fun i post -> forall j. post j)
 let tactic (a:Type) = unit -> Tac a
 
 (* working around #885 *)
-let _fail (a:Type) (msg:string) : _tac a = fun s0 -> Failed #a msg s0
-let fail (#a:Type) (msg:string) : tactic a = fun () -> TAC?.reflect (_fail a msg)
+let __fail (a:Type) (msg:string) : __tac a = fun s0 -> Failed #a msg s0
+let fail (#a:Type) (msg:string) : tactic a = fun () -> TAC?.reflect (__fail a msg)
 
 let or_else (#a:Type) (t1:tactic a) (t2:tactic a)
         : tactic a
@@ -129,10 +125,10 @@ let or_else (#a:Type) (t1:tactic a) (t2:tactic a)
 // TODO: forgot the underscore in result and F* blew up,
 // didn't mention a undefined "result". bug?
 abstract 
-let by_tactic (t:state -> _result unit) (a:Type) : Type = a
+let by_tactic (t:state -> __result unit) (a:Type) : Type = a
 
 // TODO: generalize to any type
-let reify_tactic (t:tactic unit) : _tac unit =
+let reify_tactic (t:tactic unit) : __tac unit =
   fun s -> reify (t ()) s
 
 // Must run with tactics off, as it will otherwise try to run `by_tactic
@@ -145,27 +141,27 @@ let assert_by_tactic (t:tactic unit) (p:Type)
   = ()
 #reset-options ""
 
-  // TODO: naming convention.. underscore before or after?
+// TODO: naming convention.. underscore before or after?
 
-assume private val binders_of_env_ : env -> binders
-let binders_of_env (e:env) : tactic binders = fun () -> binders_of_env_ e
+assume private val __binders_of_env : env -> binders
+let binders_of_env (e:env) : tactic binders = fun () -> __binders_of_env e
 
-assume private val type_of_binder_: binder -> term 
-let type_of_binder (b:binder) : tactic term = fun () -> type_of_binder_ b
+assume private val __type_of_binder: binder -> term 
+let type_of_binder (b:binder) : tactic term = fun () -> __type_of_binder b
 
-assume private val term_eq_ : term -> term -> bool
-let term_eq t1 t2 : tactic bool = fun () ->  term_eq_ t1 t2
+assume private val __term_eq : term -> term -> bool
+let term_eq t1 t2 : tactic bool = fun () ->  __term_eq t1 t2
 
-assume private val embed  : #a:Type -> a -> term
-let quote #a (x:a) : tactic term = fun () -> embed x
+assume private val __embed  : #a:Type -> a -> term
+let quote #a (x:a) : tactic term = fun () -> __embed x
 
 //This primitive provides a way to destruct a term as a formula
 //TODO: We should add a formula_as_term also
-assume private val term_as_formula_ : term -> option formula
-let term_as_formula t : tactic (option formula) = fun () -> term_as_formula_ t
+assume private val __term_as_formula : term -> option formula
+let term_as_formula t : tactic (option formula) = fun () -> __term_as_formula t
 
-assume val inspect_ : term -> option term_view
-let inspect t : tactic term_view = fun () -> match inspect_ t with
+assume val __inspect : term -> option term_view
+let inspect t : tactic term_view = fun () -> match __inspect t with
                                              | Some x -> x
                                              | None -> fail "inspect failed, possibly unknown syntax" ()
 
@@ -174,59 +170,59 @@ let inspect t : tactic term_view = fun () -> match inspect_ t with
    E.g., forall_intros could be an application of 
          FStar.Classical.forall_intro
  *)         
-assume private val forall_intros_: _tac binders
-let forall_intros : tactic binders = fun () -> TAC?.reflect forall_intros_
+assume private val __forall_intros: __tac binders
+let forall_intros : tactic binders = fun () -> TAC?.reflect __forall_intros
 
-assume private val implies_intro_: _tac binder
-let implies_intro : tactic binder = fun () -> TAC?.reflect implies_intro_
+assume private val __implies_intro: __tac binder
+let implies_intro : tactic binder = fun () -> TAC?.reflect __implies_intro
 
-assume private val trivial_  : _tac unit
-let trivial : tactic unit = fun () -> TAC?.reflect trivial_
+assume private val __trivial  : __tac unit
+let trivial : tactic unit = fun () -> TAC?.reflect __trivial
 
-assume private val revert_  : _tac unit
-let revert : tactic unit = fun () -> TAC?.reflect revert_
+assume private val __revert  : __tac unit
+let revert : tactic unit = fun () -> TAC?.reflect __revert
 
-assume private val clear_   : _tac unit
-let clear : tactic unit = fun () -> TAC?.reflect clear_
+assume private val __clear   : __tac unit
+let clear : tactic unit = fun () -> TAC?.reflect __clear
 
-assume private val split_   : _tac unit
-let split : tactic unit = fun () -> TAC?.reflect split_
+assume private val __split   : __tac unit
+let split : tactic unit = fun () -> TAC?.reflect __split
 
-assume private val merge_   : _tac unit
-let merge : tactic unit = fun () -> TAC?.reflect merge_
+assume private val __merge   : __tac unit
+let merge : tactic unit = fun () -> TAC?.reflect __merge
 
 // TODO: isn't this is unsound if b is not the environment? I think so but couldn't quickly come up with a contradiction
-assume private val rewrite_ : binder -> _tac unit
-let rewrite (b:binder) : tactic unit = fun () -> TAC?.reflect (rewrite_ b)
+assume private val __rewrite : binder -> __tac unit
+let rewrite (b:binder) : tactic unit = fun () -> TAC?.reflect (__rewrite b)
 
-assume private val smt_     : _tac unit
-let smt : tactic unit = fun () -> TAC?.reflect smt_
+assume private val __smt     : __tac unit
+let smt : tactic unit = fun () -> TAC?.reflect __smt
 
-assume private val visit_   : _tac unit -> _tac unit
-let visit (f:tactic unit) : tactic unit = fun () -> TAC?.reflect (visit_ (reify_tactic f))
+assume private val __visit   : __tac unit -> __tac unit
+let visit (f:tactic unit) : tactic unit = fun () -> TAC?.reflect (__visit (reify_tactic f))
 
-assume private val focus_: _tac unit -> _tac unit
-let focus (f:tactic unit) : tactic unit = fun () -> TAC?.reflect (focus_ (reify_tactic f))
+assume private val __focus: __tac unit -> __tac unit
+let focus (f:tactic unit) : tactic unit = fun () -> TAC?.reflect (__focus (reify_tactic f))
 
-(* could be implemented using focus_ *)
-assume private val seq_ : _tac unit -> _tac unit -> _tac unit
+(* could be implemented using __focus *)
+assume private val __seq : __tac unit -> __tac unit -> __tac unit
 let seq (f:tactic unit) (g:tactic unit) : tactic unit = fun () -> 
-  TAC?.reflect (seq_ (reify_tactic f) (reify_tactic g))
+  TAC?.reflect (__seq (reify_tactic f) (reify_tactic g))
 
-assume private val exact_ : term -> _tac unit
-let exact (t:tactic term) : tactic unit = fun () -> let tt = t () in TAC?.reflect (exact_ tt)
+assume private val __exact : term -> __tac unit
+let exact (t:tactic term) : tactic unit = fun () -> let tt = t () in TAC?.reflect (__exact tt)
 
-assume private val apply_lemma_ : term -> _tac unit
-let apply_lemma (t:tactic term) : tactic unit = fun () -> let tt = t () in TAC?.reflect (apply_lemma_ tt)
+assume private val __apply_lemma : term -> __tac unit
+let apply_lemma (t:tactic term) : tactic unit = fun () -> let tt = t () in TAC?.reflect (__apply_lemma tt)
 
-assume val print_ : string -> _tac unit
-let print (msg:string) : tactic unit = fun () -> TAC?.reflect (print_ msg)
+assume val __print : string -> __tac unit
+let print (msg:string) : tactic unit = fun () -> TAC?.reflect (__print msg)
 
-assume val grewrite_ : term -> term -> _tac unit
+assume val __grewrite : term -> term -> __tac unit
 let grewrite (e1:tactic term) (e2:tactic term) : tactic unit =
     fun () -> let t1 = e1 () in
               let t2 = e2 () in
-              TAC?.reflect (grewrite_ t1 t2)
+              TAC?.reflect (__grewrite t1 t2)
 
 let tret (#a:Type) (x:a) : tactic a =
     fun () -> x
@@ -239,13 +235,13 @@ let tbind' (#a:Type) (#b:Type) (t : tactic a) (f : tactic b) : tactic b =
 
 // For some reason, a direct definition fails.
 let revert_all (bs:binders) : tactic unit =
-    let rec _revert_all (bs:binders) : Tac unit =
+    let rec __revert_all (bs:binders) : Tac unit =
       match bs with
       | [] -> ()
-      | _::tl -> let _ = revert () in _revert_all tl
-    in fun () -> _revert_all bs
+      | _::tl -> let _ = revert () in __revert_all tl
+    in fun () -> __revert_all bs
 
-let get : tactic state = fun () -> TAC?._get ()
+let get : tactic state = fun () -> TAC?.__get ()
 
 let cur_goal : tactic goal = fun () ->
   let goals, _ = get () in
@@ -262,6 +258,13 @@ let destruct_equality_implication (t:term) : tactic (option (formula * term)) = 
      | _ -> None)
   | _ -> None
 
+// TODO: aux isn't used. wtf?
+// in this one, if the return type is "tactic unit", it complains
+// about not being able to show a decreasing order. again wtf?
+let rec user_visit (callback:tactic unit) : unit -> Tac unit
+    = fun () ->
+         or_else callback (user_visit callback) ()
+
 // TODO: Needs to be unit -> Tac unit since it's a let rec.
 let rec simplify_eq_implication : unit -> Tac unit
   = fun () ->
@@ -272,38 +275,7 @@ let rec simplify_eq_implication : unit -> Tac unit
       let eq_h = implies_intro () in  // G, eq_h:x=e |- P
       rewrite eq_h (); // G, eq_h:x=e |- P[e/x]
       clear ();     // G |- P[e/x]
-      visit simplify_eq_implication ()
-
-// TODO: aux isn't used. wtf?
-// in this one, if the return type is "tactic unit", it complains
-// about not being able to show a decreasing order. again wtf?
-let rec user_visit (callback:tactic unit) : unit -> Tac unit
-    = fun () ->
-         let aux : tactic unit = fun () ->
-           let context, goal_t = cur_goal () in
-           match term_as_formula goal_t () with
-           | None -> smt ()
-           | Some (Exists _ _) -> //not yet handled
-             ()
-
-           | Some (Forall xs body) ->
-             let binders = forall_intros () in
-             let _ = user_visit callback () in
-             revert_all binders ()
-
-           | Some (And t1 t2) ->
-             let _ = seq split (user_visit callback) () in
-             merge ()
-
-           | Some (Implies t1 t2) ->
-             let h = implies_intro () in
-             let _ = user_visit callback () in
-             revert ()
-
-           | _ ->
-             or_else trivial smt ()
-         in
-         or_else callback (user_visit callback) ()
+      user_visit simplify_eq_implication ()
 
 let rec try_rewrite_equality (x:term)
                              (bs:binders)
